---
title:  "Sum to Product"
date: 2024-6-27 17:22:24 +0800
categories: 
---
## Theorem
 
$$ 
\begin{equation}
\sin\alpha+\sin\beta = 2\sin(\frac{\alpha+\beta}{2})\cos(\frac{\alpha-\beta}{2}) \\
\sin\alpha-\sin\beta = 2\cos(\frac{\alpha+\beta}{2})\sin(\frac{\alpha-\beta}{2}) \\ 
\cos\alpha+\cos\beta = 2\cos(\frac{\alpha+\beta}{2})\cos(\frac{\alpha-\beta}{2}) \\
\cos\alpha-\cos\beta = -2\sin(\frac{\alpha+\beta}{2})\sin(\frac{\alpha-\beta}{2}) \\
\tan\alpha+\tan\beta = \frac{\sin(\alpha+\beta)}{\cos\alpha\cos\beta} \\
\tan\alpha-\tan\beta = \frac{\sin(\alpha-\beta)}{\cos\alpha\cos\beta} \\
\end{equation}

$$